

7. Жителуиба

[1] Да се покаже, че $(\vec{a} \times \vec{b}) \times (\vec{c} \times \vec{d}) = \langle \vec{a}, \vec{b}, \vec{d} \rangle \vec{c} - \langle \vec{a}, \vec{b}, \vec{c} \rangle \vec{d}$

$$\textcircled{1} \underbrace{(\vec{a} \times \vec{b})}_{2. \vec{e}} \times \underbrace{(\vec{c} \times \vec{d})}_{1. \vec{e}} = (\vec{a} \times \vec{b}) \times \vec{c} = \vec{b} \langle \vec{a}, \vec{c} \rangle - \vec{a} \langle \vec{b}, \vec{c} \rangle$$

$$= \vec{b} \langle \vec{a}, \vec{c} \rangle - \vec{a} \langle \vec{b}, \vec{c} \rangle =$$

$$= \vec{b} \langle \vec{a}, \vec{c} \rangle \vec{d} - \vec{a} \langle \vec{b}, \vec{c} \rangle \vec{d} \rightarrow \text{Не работи}$$

$$\textcircled{2} \rightarrow \vec{c} \times (\vec{c} \times \vec{d}) = \vec{c} \langle \vec{c}, \vec{d} \rangle - \vec{d} \langle \vec{c}, \vec{c} \rangle = \vec{c} \langle \vec{a}, \vec{b}, \vec{d} \rangle - \vec{d} \langle \vec{a}, \vec{b}, \vec{c} \rangle \quad \checkmark$$

[2] Да се покаже, че $\langle \vec{a} \times \vec{b}, \vec{b} \times \vec{c}, \vec{c} \times \vec{a} \rangle = \langle \vec{a}, \vec{b}, \vec{c} \rangle^2$

$$\textcircled{1} \langle \vec{a} \times \vec{b}, \vec{b} \times \vec{c}, \vec{c} \times \vec{a} \rangle = \langle \vec{a} \times \vec{b}, \underbrace{(\vec{b} \times \vec{c}) \times (\vec{c} \times \vec{a})}_{\vec{a}} \rangle =$$

$$= \langle \vec{a} \times \vec{b}, \vec{d} \times (\vec{c} \times \vec{a}) \rangle = \langle \vec{a} \times \vec{b}, \vec{c} \langle \vec{d}, \vec{a} \rangle - \vec{a} \langle \vec{d}, \vec{c} \rangle \rangle =$$

$$= \langle \vec{a} \times \vec{b}, \vec{c} \underbrace{\langle \vec{d}, \vec{a} \rangle}_{\text{нуло}} \rangle - \langle \vec{a} \times \vec{b}, \vec{a} \underbrace{\langle \vec{d}, \vec{c} \rangle}_{\text{нуло}} \rangle =$$

$$= \langle \vec{d}, \vec{a} \rangle \langle \vec{a} \times \vec{b}, \vec{c} \rangle - \langle \vec{d}, \vec{c} \rangle \langle \vec{a} \times \vec{b}, \vec{a} \rangle = \langle \vec{b}, \vec{c}, \vec{a} \rangle \langle \vec{a}, \vec{b}, \vec{c} \rangle - \underbrace{\langle \vec{b}, \vec{c}, \vec{c} \rangle}_0 \langle \vec{a}, \vec{b}, \vec{a} \rangle =$$

$$= \langle \vec{a}, \vec{b}, \vec{c} \rangle \langle \vec{a}, \vec{b}, \vec{c} \rangle = \langle \vec{a}, \vec{b}, \vec{c} \rangle^2$$

[3] Да се покаже, че $\vec{a} \times [(\vec{b} \times \vec{c}) \times \vec{d}] = \langle \vec{a}, \vec{d} \rangle \vec{b} \times \vec{c} - \langle \vec{a}, \vec{b}, \vec{c} \rangle \vec{d}$

$$\textcircled{1} \vec{a} \times \underbrace{[(\vec{b} \times \vec{c}) \times \vec{d}]}_{\vec{e}} = \vec{a} \times (\vec{c} \times \vec{d}) = \vec{c} \langle \vec{a}, \vec{d} \rangle - \vec{d} \langle \vec{a}, \vec{c} \rangle =$$

$$= \vec{b} \times \vec{c} \langle \vec{a}, \vec{d} \rangle - \vec{d} \langle \vec{a}, \vec{b}, \vec{c} \rangle$$

[4] Да се покаже $(\vec{a} \times \vec{b})^2 (\vec{a} \times \vec{c})^2 - \langle \vec{a} \times \vec{b}, \vec{a} \times \vec{c} \rangle^2 = |\vec{a}|^2 \langle \vec{a}, \vec{b}, \vec{c} \rangle^2$

$$MC - (|\vec{a} \times \vec{b}| |\vec{a} \times \vec{c}| - \langle \vec{a} \times \vec{b}, \vec{a} \times \vec{c} \rangle) (|\vec{a} \times \vec{b}| |\vec{a} \times \vec{c}| + \langle \vec{a} \times \vec{b}, \vec{a} \times \vec{c} \rangle) =$$

$$= (|\vec{a}| |\vec{b}| \sin \varphi(\vec{a}, \vec{b}) |\vec{a}| |\vec{c}| \sin \varphi(\vec{a}, \vec{c}) - \langle \vec{a}, \vec{b}, \vec{c} \rangle) (|\vec{a}| |\vec{b}| \sin \varphi(\vec{a}, \vec{b}) |\vec{a}| |\vec{c}| \sin \varphi(\vec{a}, \vec{c}) + \langle \vec{a}, \vec{b}, \vec{c} \rangle) \quad \vec{a}, \vec{b}, \vec{c}$$

$$\langle \vec{a}, \vec{b} \times \vec{c} \rangle = \langle \vec{a}, \vec{b} \times (\vec{a} \times \vec{c}) \rangle = \langle \vec{a}, \vec{a} \times \vec{c} \times \vec{b} \rangle = \langle \vec{c} \times \vec{b}, \vec{a} \rangle = |\vec{a}|^2 \langle \vec{b}, \vec{c} \rangle = \langle \vec{b}, \vec{a} \rangle \langle \vec{a}, \vec{c} \rangle = |\vec{a}| |\vec{b}| |\vec{c}| \cos \varphi(\vec{b}, \vec{c}) = |\vec{a}| |\vec{b}| |\vec{c}| \cos \varphi(\vec{a}, \vec{b}) \cos \varphi(\vec{a}, \vec{c})$$